theories/AlmostStlc/Compatibility.v
@@ -1,0 +1,119 @@
+Require Export TypedVar.
+Require Export SyntaxSeq.
+Require Export SmallStepSeq.
+Require Export DenotationFacts.
+Require Export DenotationSeq.
+Require Export TypesEquiv.
+Require Export MapEFacts.
+Import List.ListNotations.
+Open Scope list_scope.
+From Equations Require Import Equations Signature.
+Require Import Coq.Program.Equality.
+Require Import ExtLib.Structures.Monad.
+Require Import Coq.Relations.Relation_Operators.
+Import MonadNotation.
+Local Open Scope monad_scope.
+Require Export SemanticsFactsSeq.
+Require Export CallMrecFacts.
+Require Export SemanticsFactsSeq2.
+Require Import Lia.
+Require Import Coq.Classes.Morphisms.
+Require Export ClosingSubst.
+Require Export LogicalApprox.
+
+Definition denote_comp_type t Γ MR : Type :=
+  denote_ctx Γ -> mtree (denote_mfix_ctx MR) (denote_type t).
+
+Definition comp_bind {Γ MR t1 t2}
+           (m1 : denote_comp_type t1 Γ MR)
+           (m2 : denote_comp_type t2 (t1 :: Γ) MR) :
+  denote_comp_type t2 Γ MR :=
+  fun hyps => x <- m1 hyps;; m2 (x, hyps).
+  
+(* 
+
+   Lemma that is typically true according to nick
+   e1 --> e1' => e1' <=j e2 => e1 <=(j+1) e2
+
+   think about if this makes sense, especially in light of
+   whether you decrement steps in the ret case 
+
+*)
+
+
+(* this might need to be an inductive proof *)
+Lemma let_compat Γ MR t1 t2 
+      (m1 : denote_comp_type t1 Γ MR) (m2 : denote_comp_type t2 (t1 :: Γ) MR)
+      (c1 : comp t1 Γ MR) (c2 : comp t2 (t1 :: Γ) MR)
+  : comp_rel m1 c1 -> comp_rel m2 c2 ->
+    comp_rel (comp_bind m1 m2) (comp_let c1 c2).
+Proof.
+  intros Hmc1 Hmc2. intros n hyps ρ Hhρ.
+  constructor. intros Hn. specialize (Hmc1 n hyps ρ Hhρ) as Hmc1n.
+  inversion Hmc1n. intros. subst. destruct (H Hn) as [Hretmc1 Hstuckmc1]. clear H.
+  split.
+  - intros vv2 Hvv2. unfold comp_bind in Hvv2.
+    assert (exists vv1, comp_equiv_rutt (m1 hyps) (ret vv1)).
+    admit.
+    destruct H as [vv1 Hvv1]. specialize (Hretmc1 vv1 Hvv1).
+    destruct Hretmc1 as [v1 [Hv11 Hv12]].
+    (* maybe steps should not decrement in the ret case? 
+       I am concerned that might break other things  *) 
+    assert (Hhρ' : closing_subst_approx n (t1 :: Γ) (vv1, hyps) (v1, ρ)).
+    constructor; auto.
+    assert (comp_equiv_rutt (m2 (vv1, hyps)) (ret vv2)).
+    admit.
+    specialize (Hmc2 n (vv1, hyps) (v1, ρ) Hhρ') as Hmc2n.
+    inversion Hmc2n. 
+    destruct (H0 Hn) as [Hretmc2 Hstuckmc2]. clear H0.
+    apply Hretmc2 in H.
+    destruct H as [v2 [Hv21 Hv22]]. exists v2. split; auto.
+    admit.
+  - intros. rename H into Hcall.
+    (* start tomorrow by stating this lemma assertion  *)
+    assert (Hcase :
+             (exists k', comp_equiv_rutt (m1 hyps) (vv <- call_term x xR vvcall;; k' vv))
+               \/
+             (exists vv1, comp_equiv_rutt (m1 hyps) (ret vv1) /\ 
+                       comp_equiv_rutt (m2 (vv1, hyps)) (vv <- call_term x xR vvcall;; k vv)
+           )).
+    admit.
+    destruct Hcase as [[k' Hk'] | [vv1 [Hvv11 Hvv12] ]].
+    + apply Hstuckmc1 in Hk' as Hcall'.
+      destruct Hcall' as [vcall [E [c' [Hvcall [HE1 [HE2 HE3 ]] ]]] ].
+       (* figure out how to construct the evaluation context that is morally this
+          perhaps close_comp is not general enough 
+          needs to be a more general substitution?
+
+
+          
+        *) 
+      eexists. eexists. eexists. split; eauto. split; [ | split]; eauto.
+      * admit.
+      * admit.
+      * intros. apply HE3 in H0; auto.
+        (* concerned about this part 
+           k vvret = k' vvret ;; m2 kyps
+           use that to substitute in
+           if I have an induction hypothesis according to <
+           then maybe I can continue
+           this is starting to look sketchy, but not necessarily unsalvageable
+
+           also might be easier and sufficient to prove approx_comp composes with
+           bind/let at a fixed j'
+           
+
+         *)
+        admit.
+   + apply Hretmc1 in Hvv11 as Hvv13. destruct Hvv13 as [v1 [Hv11 Hv12]].
+     (* lost the thread a bit on this one *)
+     assert (Hhρ' : closing_subst_approx n (t1 :: Γ) (vv1, hyps) (v1, ρ)).
+     constructor; auto. specialize (Hmc2 _ _ _ Hhρ').
+     inversion Hmc2. specialize (H Hn). destruct H as [Hretmc2 Hstuckmc2].
+     subst. apply Hstuckmc2 in Hvv12 as Hvv13.
+     destruct Hvv13 as [vcall [E [c' [Hvcall [HE1 [HE2 HE3 ]] ]]] ].
+     exists vcall. eexists. eexists. split; [ auto | split ]; [ | split].
+     * admit.
+     * admit.
+     * auto.
+Admitted.
