theories/AlmostStlc/LogicalApprox.v
@@ -1,0 +1,306 @@
+Require Export TypedVar.
+Require Export SyntaxSeq.
+Require Export SmallStepSeq.
+Require Export DenotationFacts.
+Require Export DenotationSeq.
+Require Export TypesEquiv.
+Require Export MapEFacts.
+Import List.ListNotations.
+Open Scope list_scope.
+From Equations Require Import Equations Signature.
+Require Import Coq.Program.Equality.
+Require Import ExtLib.Structures.Monad.
+Require Import Coq.Relations.Relation_Operators.
+Import MonadNotation.
+Local Open Scope monad_scope.
+Require Export SemanticsFactsSeq.
+Require Export CallMrecFacts.
+Require Export SemanticsFactsSeq2.
+Require Import Lia.
+Require Import Coq.Classes.Morphisms.
+Require Export ClosingSubst.
+
+Definition valid_denote {t} (vv : denote_type t) : Prop :=
+  types_equiv t vv vv.
+
+Inductive approx_comp {t MR} (j : nat) (R : nat -> forall t, denote_type t -> closed_value t -> Prop) :
+           forall (m : mtree (denote_mfix_ctx MR) (denote_type t)) (c : comp t [] MR), Prop := 
+  approx_comp_intro m c : (j > 1 ->
+                                (forall (vv : denote_type t), comp_equiv_rutt m (ret vv) -> exists v, eval_rel_stuck c (inl v) /\ R j t vv v) /\
+                                (forall (tin tout : type) Rcall (xR : var Rcall MR) (x : var (tin, tout) Rcall) (vvcall : denote_type tin) k,
+                                    comp_equiv_rutt m (vv <- call_term x xR vvcall;; k vv) ->
+                                    exists (vcall : closed_value tin) (E : eval_context t MR (inr (SmallStepSeq.callv xR x vcall) ) true) (c' : comp t [] MR),
+                                      R j tin vvcall vcall /\ 
+                                      eval_rel_stuck c (inr c') /\ stuck_call c' ((SmallStepSeq.callv xR x vcall)) E /\
+                                        (forall j' (vvret : denote_type tout) (vret : closed_value tout), j' < j -> 
+                                          R j' tout vvret vret ->
+                                          approx_comp j' R (k vvret) (subst_eval_context E (comp_ret vret)))))
+
+                                -> approx_comp j R m c.
+
+
+
+Inductive log_rel_list {t} (R : Rel (denote_type t) (closed_value t) ) : 
+   denote_type (List t) -> closed_value (List t)  -> Prop := 
+ | log_rel_list_nil : log_rel_list R nil val_nil
+ | log_rel_list_cons vvh vh vvt vt : R vvh vh -> log_rel_list R vvt vt ->
+                                     log_rel_list R (cons vvh vvt) (val_cons vh vt) 
+.
+
+(* well founded relation over nat * type *)
+(* Coq.Wellfounded.Union 
+   
+
+*)
+
+(* need to make a step indexed version *)
+Derive Subterm for type.
+
+Definition log_rel_dec : Rel (nat * type) (nat * type) := slexprod nat type lt type_subterm.
+
+Instance log_rel_dec_wf : WellFounded log_rel_dec.
+Proof.
+  apply Lexicographic_Product.wf_slexprod.
+  - apply PeanoNat.Nat.lt_wf_0.
+  - apply well_founded_type_subterm.
+Qed.
+
+Equations approx_val (n : nat) (t : type) (vv : denote_type t) (v : closed_value t) : Prop by wf (n,t) log_rel_dec := {
+  approx_val 0 _ _ _ := True;
+  approx_val (S m') Nat n (val_const m) := n = m;
+  approx_val (S m) (Pair t1 t2) (vv1, vv2) (val_pair v1 v2)  := approx_val (S m) t1 vv1 v1 /\ approx_val (S m) t2 vv2 v2;
+  approx_val (S m) (List t) l vl := log_rel_list (fun vv v => approx_val (S m) t vv v) l vl;
+  approx_val (S m) (Arrow t1 MR t2) f (val_abs c) := 
+    forall vv v m' (H : m' < S m), valid_denote vv -> approx_val m' t1 vv v -> 
+                              approx_comp m' (fun n t v vv => forall (H : n < S m), 
+                                                  approx_val n t v vv) (f vv) (subst_comp_cons c v) 
+}.
+Next Obligation. 
+  right. constructor. constructor.
+Qed.
+Next Obligation.
+  right. constructor. constructor.
+Qed.
+Next Obligation.
+  right. constructor. constructor.
+Qed.
+Next Obligation.
+  left. auto.
+Qed.
+Next Obligation.
+  left. auto.
+Qed.
+
+
+Lemma lower_approx_comp_aux1 : forall (P : nat -> Prop) n t MR c m R1 R2,
+    P n ->
+    (forall n m, n <= m -> P m -> P n) ->
+    (forall n' t vv v, P n' -> (R1 n' t vv v <-> R2 n' t vv v)) ->
+    approx_comp (t := t) (MR := MR) n R1 m c -> 
+    approx_comp n R2 m c.
+Proof.
+  intros P n.
+  induction n as [ n IHn ] using (well_founded_induction lt_wf).
+  (* - intros t MR c m R1 R2 Hn Hclosed HR Hcm.
+    econstructor. intros. lia. *)
+  intros t MR c m R1 R2 Hn Hclosed HR Hcm.
+  dependent induction Hcm.
+  constructor. intros Hn'. specialize (H Hn').
+  destruct H as [Hret Hstuck].
+  split.
+  - intros vv Hvv. apply Hret in Hvv. decompose record Hvv. eexists. split; eauto.
+    apply HR; auto.
+  - intros. apply Hstuck in H. destruct H as [vcall [E [c' [H1 [H2 [H3 H4]]]]]].
+    exists vcall, E, c'.
+    split; try split; try split; auto.
+    + apply HR; auto. (* apply Hclosed with (n := n-1) (m := n); auto. lia. *)
+    + intros j' vvret vret Hvret Hj'. destruct n; cbn. constructor. intros. lia.
+      eapply IHn; eauto. 
+      eapply H4. lia. eapply HR. eapply Hclosed; try apply Hn. lia. auto.
+Qed.
+
+Lemma lower_approx_val_aux : forall n t v vv, approx_val (S n) t vv v -> approx_val n t vv v.
+Proof.
+  intros n. induction n; intros.
+  - simp approx_val. auto.
+  - induction t.
+    + red in v. dependent destruction v; try inversion x. simp approx_val in H.
+      simp approx_val.
+    + red in v. clear - H IHt. dependent induction v; try inversion x.
+      * simp approx_val. simp approx_val in H.
+        inversion H. subst. constructor.
+      * simp approx_val. simp approx_val in H. inversion H. subst.
+        inj_existT. subst.
+        constructor. apply IHt. auto.
+        specialize (IHv2 t v2 eq_refl eq_refl JMeq_refl vvt).
+        simp approx_val in IHv2.
+    + red in v. dependent destruction v; try inversion x.
+      destruct vv as [vv1 vv2]. simp approx_val in H. simp approx_val.
+      destruct H. split; auto.
+    + red in v. dependent destruction v; try inversion x.
+      rename vv into f. simp approx_val in H. simp approx_val.
+      intros vv v m' Hm' Hvv Hv. eapply H in Hv; eauto.
+      eapply lower_approx_comp_aux1 with (P := fun m' => m' < S n); intros; eauto.
+      lia. simpl.
+      split; intros; apply H1; lia.
+Qed.
+
+Lemma lower_approx_comp_aux2 : forall n t MR c m R,
+    (forall n m t v vv, n < m -> (R m t v vv : Prop) -> R n t v vv) ->
+    approx_comp (t := t) (MR := MR) (S n) R c m ->
+    approx_comp n R c m.
+Proof.
+  intros n. induction n.
+  { intros. constructor. intros. lia. }
+  intros t MR c m R HR Hcm.
+  dependent destruction Hcm. constructor. intros Hn.
+  assert (Hn' : S (S n) > 1). lia.
+  specialize (H Hn'). destruct H as [Hret Hstuck].
+  split.
+  - intros vv Hvv. eapply Hret in Hvv as [v [Hv1 Hv2]].
+    eexists. split; eauto. (* eapply HR; try apply Hv2. lia. *)
+  - intros tin tout Rcall xR x vvcall k Hca. apply Hstuck in Hca.
+    destruct Hca as [vcall [E [c' [HE1 [HE2 [HE3 HE4]]]]]].
+    exists vcall, E, c'. repeat (split; auto).
+    eapply HR; try apply HE1. lia.
+Qed.
+
+
+Lemma lower_approx_comp_aux3 n j t MR c m : 
+  n < j->
+  approx_comp n approx_val m c ->
+  approx_comp (t := t) (MR := MR) n
+              (fun n t vv v => forall (H : n < j), approx_val n t vv v) m c.
+Proof.
+  intros. eapply lower_approx_comp_aux1 with (P := fun n => n < j); eauto.
+  lia. intros. simpl. split; intros; auto.
+Qed.
+
+Lemma lower_approx_val : forall n m, n < m -> forall t vv v, approx_val m t vv v -> approx_val n t vv v.
+Proof.
+  intros n m Hnm. red in Hnm. dependent induction Hnm.
+  - intros. apply lower_approx_val_aux. auto.
+  - intros. apply lower_approx_val_aux in H. auto.
+Qed.
+
+Lemma lower_approx_comp : forall n j, n < j -> forall t MR c m R,
+    (forall n m t v vv, n < m -> (R m t v vv : Prop) -> R n t v vv) ->
+    approx_comp (t := t) (MR := MR) j R c m ->
+    approx_comp n R c m.
+Proof.
+  intros n j Hnj. red in Hnj. dependent induction Hnj.
+  - intros. apply lower_approx_comp_aux2; auto.
+  - intros. apply lower_approx_comp_aux2 in H0; auto.
+Qed.
+
+(* may also need that vv is valid *)
+Inductive closing_subst_approx (n : nat) : forall Γ, denote_ctx Γ -> closing_subst Γ ->  Prop :=
+  | closing_subst_approx_nil : closing_subst_approx n nil tt tt
+  | closing_subst_approx_cons t Γ v ρ vv hyps : 
+    approx_val n t v vv -> closing_subst_approx n Γ ρ hyps ->
+    closing_subst_approx n (t :: Γ) (v, ρ) (vv, hyps)
+.
+
+Lemma lower_closing_subst_approx:
+  forall (n m : nat) (Γ : ctx) (ρ : closing_subst Γ) (hyps : denote_ctx Γ),
+    closing_subst_approx n Γ hyps ρ ->
+    m < n -> closing_subst_approx m Γ hyps ρ.
+Proof.
+  intros n m Γ ρ hyps H Hm.
+  generalize dependent Γ. intros Γ. induction Γ.
+  intros. destruct ρ. destruct hyps. constructor.
+  intros [v ρ] [vv hyps] H. dependent destruction H.
+  constructor; auto. eapply lower_approx_val; eauto.
+Qed.
+
+
+Lemma proper_approx_aux : forall n,
+    (forall t v vv1 vv2, types_equiv t vv1 vv2 -> approx_val n t vv1 v -> approx_val n t vv2 v) /\
+    (forall t MR c m1 m2, comp_equiv_rutt (t := t) (MR := MR) m1 m2 -> 
+       approx_comp n approx_val m1 c -> approx_comp n approx_val m2 c).
+Proof.
+  intros n. induction n as [ n IHn ] using (well_founded_induction lt_wf).
+  assert (IHv : forall y, y < n -> 
+           (forall (t : vtype) (v : closed_value t) (vv1 vv2 : denote_type t),
+         types_equiv t vv1 vv2 -> approx_val y t vv1 v -> approx_val y t vv2 v)).
+  { intros. apply IHn in H. destruct H. eauto. }
+  assert (IHc : forall y, y < n -> 
+           (forall t MR c m1 m2, comp_equiv_rutt (t := t) (MR := MR) m1 m2 -> 
+       approx_comp y approx_val m1 c -> approx_comp y approx_val m2 c)).
+  { intros. apply IHn in H. destruct H. eauto. }
+  clear IHn.
+  split; intros.
+  - destruct n. simp approx_val. auto.
+    induction t.
+    + red in v. dependent destruction v; try inversion x. simp approx_val in *.
+      simp types_equiv in H. subst. auto.
+    + simp approx_val. simp approx_val in H0. 
+      red in v. clear - H H0 IHt. dependent induction v; try inversion x.
+      * dependent destruction H0. simp types_equiv in H. dependent destruction H.
+        constructor.
+      * dependent destruction H0. simp types_equiv in H.
+        dependent destruction H. rename b into vv1. rename l2 into vv2.
+        constructor; eauto.
+        eapply IHv2; eauto. simp types_equiv.
+    + red in v. dependent destruction v; try inversion x.
+      simp types_equiv in H. destruct vv1 as [vv11 vv12]. destruct vv2 as [vv21 vv22].
+      dependent destruction H. cbn in *. simp approx_val in *.
+      destruct H0. split; eauto.
+    + red in v. dependent destruction v; try inversion x.
+      rename vv1 into f1. rename vv2 into f2. simp types_equiv in H. simp approx_val.
+      intros vv v m' Hm' Hvv Hv.
+      apply H in Hvv as Hvv'.
+      eapply lower_approx_comp_aux1 with (P := fun m' => m' < S n) (R1 := approx_val); eauto. intros. lia.
+      intros. split; intros; auto.
+      eapply IHc; eauto. simp approx_val in H0. 
+      eapply lower_approx_comp_aux1 with (P := fun m' => m' < S n); eauto. lia.
+      intros. simpl. split; intros; auto.
+  - constructor. intros. inversion H0. subst. specialize (H2 H1) as [Hret Hstuck].
+    split.
+    + intros. rewrite <- H in H2. eapply Hret. auto.
+    + intros. rewrite <- H in H2. apply Hstuck in H2. eauto.
+Qed.
+
+#[local] Instance proper_approx_val {n t} : Morphisms.Proper (types_equiv t ==> eq ==> Basics.flip Basics.impl) (approx_val n t).
+Proof.
+  repeat intro. subst. destruct (proper_approx_aux n). eapply H0; eauto. symmetry. auto.
+Qed.
+
+#[local] Instance proper_approx_comp {n t MR} : Morphisms.Proper (comp_equiv_rutt (t := t) (MR := MR)  ==> eq ==> Basics.flip Basics.impl) (approx_comp n approx_val).
+Proof.
+  repeat intro. subst. destruct (proper_approx_aux n). eapply H2; eauto. symmetry. auto.
+Qed.
+
+
+(* needs to include this new bodies steps t *)
+Equations log_rel_bodies_step {MR R1 R2} 
+          (n : nat)
+          (dbodies : forall arg : denote_call_frame R2, mtree (denote_mfix_ctx (R1 :: MR)) (encodes arg))
+          (bodies : mfix_bodies [] MR R1 R2) : Prop :=
+  log_rel_bodies_step _ f mfix_bodies_nil := True;
+  log_rel_bodies_step n f (mfix_bodies_cons cbody bodies) :=
+   approx_val n (Arrow t1 (R1 :: MR) t2) (fun vv => f (inl vv)) (val_abs cbody) /\
+      log_rel_bodies_step n (fun vv => f (inr vv)) bodies.
+
+
+Definition comp_rel {t Γ MR} 
+           (m : denote_ctx Γ -> mtree (denote_mfix_ctx MR) (denote_type t))
+           (c : comp t Γ MR) : Prop :=
+  forall n (hyps : denote_ctx Γ) (ρ : closing_subst Γ), 
+    closing_subst_approx n Γ hyps ρ -> approx_comp n approx_val (m hyps) (close_comp Γ ρ c).
+
+Definition val_rel {t Γ MR}
+           (vm : denote_ctx Γ -> mtree (denote_mfix_ctx MR) (denote_type t))
+           (v : value t Γ) : Prop :=
+  forall n (hyps : denote_ctx Γ) (ρ : closing_subst Γ), 
+    closing_subst_approx n Γ hyps ρ -> 
+    exists vv, vm hyps ≈ ret vv /\
+            approx_val n t vv (close_value Γ ρ v).
+
+
+Definition bodies_rel {Γ MR R1 R2}
+           (dbodies : denote_ctx Γ -> forall arg : denote_call_frame R2, mtree (denote_mfix_ctx (R1 :: MR)) (encodes arg))
+           (bodies : mfix_bodies Γ MR R1 R2) : Prop :=
+  forall n (hyps : denote_ctx Γ) (ρ : closing_subst Γ), 
+    closing_subst_approx n Γ hyps ρ -> 
+     log_rel_bodies_step n (dbodies hyps) (close_bodies Γ ρ bodies).
