theories/AlmostStlc/PCF.v
@@ -1,0 +1,11 @@
+Require Export SyntaxSeq.
+
+
+Inductive pcf_term :=
+  | pcf_const (n : nat) : pcf_term
+  | pcf_nil : pcf_term
+  | pcf_cons (h t : pcf_term) : pcf_term
+  | pcf_pair (l r : pcf_term) : pcf_term
+  | pcf_abs (body : pcf_term) : pcf_term
+  | pcf_var (n : nat) : pcf_term
+.
