theories/AlmostStlc/RecursionTrace.v
@@ -1,0 +1,156 @@
+Require Export TypedVar.
+Require Export SyntaxSeq.
+Require Export SmallStepSeq.
+Require Export DenotationFacts.
+Require Export DenotationSeq.
+Require Export TypesEquiv.
+Require Export MapEFacts.
+Import List.ListNotations.
+Open Scope list_scope.
+From Equations Require Import Equations Signature.
+Require Import Coq.Program.Equality.
+Require Import ExtLib.Structures.Monad.
+Require Import Coq.Relations.Relation_Operators.
+Import MonadNotation.
+Local Open Scope monad_scope.
+Require Export SemanticsFactsSeq.
+Require Export CallMrecFacts.
+Require Export SemanticsFactsSeq2.
+Require Import Lia.
+Require Import Coq.Classes.Morphisms.
+
+From Paco Require Import paco.
+
+From ITree Require Import
+     Basics.Basics
+     Basics.Tacs
+     Basics.HeterogeneousRelations
+     Eq.Paco2.
+
+Section RecursionTrace.
+
+Context (D E : Type) `{EncodedType D} `{EncodedType E}.
+Context (bodies : forall (d : D), entree (D + E) (encodes d)).
+
+(* this is a little messy *)
+Inductive recursion_trace {A : Type} : 
+  entree (D + E) A -> list D -> entree E A -> Prop := 
+  | recursion_trace_ret_in t vv : t ≈ ret vv -> recursion_trace t [] (ret vv)
+  | recursion_trace_inr_in t (e : E) k1 k2  : 
+    t ≈ (Vis (inr e) k1) -> (forall x, interp_mrec bodies (k1 x) ≈ interp_mrec bodies (k2 x)) -> 
+    recursion_trace t [] (Vis e (fun vv => (interp_mrec bodies (k2 vv))))
+  | recursion_trace_inl_in t1 (d : D) k1 t2 l t3: 
+    t1 ≈ (Vis (inl d) k1) ->
+    t2 ≈ (bind (bodies d) k1) ->
+    recursion_trace t2 l t3 ->
+    recursion_trace t1 (d :: l) t3
+
+.
+
+
+Instance recursion_trace_eutt A : Proper (eutt eq ==> eq ==> eq ==> Basics.flip Basics.impl) (@recursion_trace A).
+Proof.
+  repeat intro. subst. generalize dependent x.
+  induction H4.
+  - constructor. rewrite H2. auto.
+  - intros. econstructor. rewrite H3. eauto. auto.
+  - intros. econstructor; eauto. rewrite H3. auto.
+Qed.
+
+Lemma recursion_trace_ret R (t : entree (D + E) R) r: 
+  interp_mrec bodies t ≈ ret r ->
+  exists (l : list D), recursion_trace t l (ret r).
+Proof.
+  intros Hret. punfold Hret. red in Hret.
+  cbn in Hret. remember (RetF r) as y.
+  remember (observe (interp_mrec bodies t)) as x.
+  assert (go _ _ x ≅ interp_mrec bodies t). subst. rewrite <- entree_eta. reflexivity.
+  clear Heqx. generalize dependent H1. revert t.
+  hinduction Hret before bodies; intros; inv Heqy.
+  - unfold interp_mrec in H1.
+    destruct (observe t) eqn : Heq; try destruct e.
+    + setoid_rewrite interp_mrec_ret in H1. apply eqit_Ret_inv in H1. subst.
+      symmetry in Heq. apply simpobs in Heq. exists []. constructor. rewrite Heq. reflexivity.
+    + setoid_rewrite interp_mrec_tau in H1. pinversion H1. inv CHECK.
+    + setoid_rewrite interp_mrec_vis_inl in H1. pinversion H1; inv CHECK.
+    + setoid_rewrite interp_mrec_vis_inr in H1. pinversion H1; inv CHECK.
+  - unfold interp_mrec in H1. destruct (observe t) eqn : Heq; try destruct e.
+    + setoid_rewrite interp_mrec_ret in H1. pinversion H1; inv CHECK. inv CHECK0.
+    + setoid_rewrite interp_mrec_tau in H1. specialize (IHHret r eq_refl t0). 
+      assert (t1 ≅ interp_mrec bodies t0). pinversion H1; try inv CHECK; try inv CHECK0.
+      apply REL. rewrite <- entree_eta in IHHret. apply IHHret in H2.
+      destruct H2 as [l Hl]. exists l. symmetry in Heq. apply simpobs in Heq.
+      rewrite <- Heq. rewrite tau_eutt. auto.
+    + setoid_rewrite interp_mrec_vis_inl in H1.
+      assert (t1 ≅ (interp_mrec bodies (x <- bodies d;; k x))).
+      pinversion H1; try inv CHECK; try inv CHECK0. auto.
+      specialize (IHHret r eq_refl (x <- bodies d;; k x)).
+      rewrite <- entree_eta in IHHret. specialize (IHHret H2).
+      destruct IHHret as [l Hl].
+      exists (d :: l). eapply recursion_trace_inl_in; eauto. 2 : reflexivity.
+      symmetry in Heq. apply simpobs in Heq. rewrite Heq. reflexivity.
+    + setoid_rewrite interp_mrec_vis_inr in H1. pinversion H1. inv CHECK0.
+Qed.
+
+
+Lemma recursion_trace_vis R (t : entree (D + E) R) e k :
+  interp_mrec bodies t ≈ Vis e (fun x => interp_mrec bodies (k x)) ->
+  exists (l : list D), recursion_trace t l (Vis e (fun x => interp_mrec bodies (k x))).
+Proof.
+  intros Hvis. punfold Hvis. red in Hvis.
+  cbn in Hvis. remember (VisF e (fun x => interp_mrec bodies (k x))) as y.
+  remember (observe (interp_mrec bodies t)) as x.
+  assert (go _ _ x ≅ interp_mrec bodies t). subst. rewrite <- entree_eta. reflexivity.
+  clear Heqx. generalize dependent H1. revert t.
+  hinduction Hvis before bodies; intros; inv Heqy.
+  - inj_existT. subst. unfold interp_mrec in H1.
+    destruct (observe t) eqn : Heq; try destruct e.
+    + setoid_rewrite interp_mrec_ret in H1. pinversion H1.
+    + setoid_rewrite interp_mrec_tau in H1. pinversion H1. inv CHECK.
+    + setoid_rewrite interp_mrec_vis_inl in H1. pinversion H1; inv CHECK.
+    + pclearbot. setoid_rewrite interp_mrec_vis_inr in H1. exists []. 
+      symmetry in Heq. apply simpobs in Heq. rewrite <- Heq.
+      assert (e0 = e). pinversion H1. auto. subst. 
+      econstructor. reflexivity. intros.
+      eapply eqit_Vis_inv in H1. Unshelve. 2: auto. rewrite <- H1. apply REL.
+  - unfold interp_mrec in H1. destruct (observe t) eqn : Heq; try destruct e0.
+    + setoid_rewrite interp_mrec_ret in H1. pinversion H1; inv CHECK. inv CHECK0.
+    + setoid_rewrite interp_mrec_tau in H1. specialize (IHHvis e k eq_refl t0). 
+      assert (t1 ≅ interp_mrec bodies t0). pinversion H1; try inv CHECK; try inv CHECK0.
+      apply REL. rewrite <- entree_eta in IHHvis. apply IHHvis in H2.
+      destruct H2 as [l Hl]. exists l. symmetry in Heq. apply simpobs in Heq.
+      rewrite <- Heq. rewrite tau_eutt. auto.
+    + setoid_rewrite interp_mrec_vis_inl in H1.
+      assert (t1 ≅ (interp_mrec bodies (x <- bodies d;; k0 x))).
+      pinversion H1; try inv CHECK; try inv CHECK0. auto.
+      specialize (IHHvis e k eq_refl (x <- bodies d;; k0 x)).
+      rewrite <- entree_eta in IHHvis. specialize (IHHvis H2).
+      destruct IHHvis as [l Hl].
+      exists (d :: l). eapply recursion_trace_inl_in; eauto. 2 : reflexivity.
+      symmetry in Heq. apply simpobs in Heq. rewrite Heq. reflexivity.
+    + setoid_rewrite interp_mrec_vis_inr in H1. pinversion H1. inv CHECK0.
+Qed.
+
+End RecursionTrace.
+
+
+Lemma call_extract (MR : mfix_ctx) (d : denote_mrec_ctx (denote_mfix_ctx MR)) : 
+  exists R (xR : var R MR) t1 t2 (x : var (t1,t2) R)  (vin : denote_type t1),
+    projT1 (call_mrec x xR vin) = d.
+Proof.
+  revert d. induction MR.
+  intros [].
+  rename a into R. intros [dR | dMR].
+  - exists R, VarZ. clear IHMR. induction R.
+    inversion dR. destruct a as [tin tout].
+    destruct dR as [vvin | ?].
+    + exists tin, tout, VarZ, vvin. simp call_mrec. rewrite call_mrec_call_frame_equation_1. auto.
+    + specialize (IHR d). destruct IHR as [t1 [t2 [x [vin H] ]] ].
+      simp call_mrec in H.
+      exists t1,t2, (VarS x), vin. simp call_mrec. rewrite call_mrec_call_frame_equation_2.
+      destruct (call_mrec_call_frame x vin). cbn in *. injection H. intros. subst. auto.
+  - specialize (IHMR dMR). destruct IHMR as [R' [xR [t1 [t2 [x [vin H]]]]]].
+    exists R', (VarS xR), t1, t2, x, vin. simp call_mrec. destruct (call_mrec x xR vin).
+    cbn in H. subst. auto.
+Qed.
+(* did I already prove this somewhere else?*)
